src/UntypedCompCombined.v
@@ -1,0 +1,74 @@
+Require Import compcert.driver.Compiler compcert.common.Errors.
+Require Import Common Monads.
+Require CompilationUnit.
+Require Import Metadata.
+Require Import CompilerUtil.
+
+Require SourceLifted Untyped8.
+Require
+    UntypedComp1
+    UntypedComp2
+    UntypedComp3
+    UntypedComp4
+    UntypedComp5
+    UntypedComp6
+    UntypedComp7
+    UntypedComp8
+.
+
+Module A := SourceLifted.
+Module B := Untyped8.
+
+Definition compile_cu {G} (cu : A.genv G * list metadata) : res (B.env * list metadata) :=
+  OK cu
+  @@ UntypedComp1.compile_cu
+  @@ UntypedComp2.compile_cu
+  @@ UntypedComp3.compile_cu
+  @@ UntypedComp4.compile_cu
+  @@ UntypedComp5.compile_cu
+  @@ UntypedComp6.compile_cu
+ @@@ UntypedComp7.compile_cu
+  @@ UntypedComp8.compile_cu
+.
+
+
+
+(*
+Require Semantics.
+
+Section Preservation.
+
+  Variable prog : A.prog_type.
+  Variable tprog : B.prog_type.
+
+  Hypothesis TRANSF : compile_cu prog = OK tprog.
+
+  Theorem fsim :
+    Semantics.forward_simulation (A.semantics prog) (B.semantics tprog).
+  Proof.
+    unfold compile_cu in TRANSF.
+    break_result_chain.
+
+    eapply Semantics.compose_forward_simulation.
+    eapply StackMachComp.fsim; try eassumption.
+
+    eapply Semantics.compose_forward_simulation.
+    eapply StackContComp.fsim; try eassumption.
+
+    eapply Semantics.compose_forward_simulation.
+    eapply StackContComp2.fsim; try eassumption.
+
+    eapply Semantics.compose_forward_simulation.
+    eapply StackContComp3.fsim; try eassumption.
+
+    eapply Semantics.compose_forward_simulation.
+    eapply StackFlatComp.fsim; try eassumption.
+
+    eapply Semantics.compose_forward_simulation.
+    eapply StackFlatterComp.fsim; try eassumption.
+
+    eapply StackFlatterComp2.fsim; try eassumption.
+  Qed.
+
+End Preservation.
+*)
